theories/gitree/weakestpre.v
@@ -159,6 +159,19 @@ Section weakestpre.
       now do 3 f_equiv.
     - reflexivity.
   Qed.
+  #[export] Instance has_substate_proper {sR : sReifier a} `{!stateG Σ}
+    `{!subReifier sR rs} : Proper ((≡) ==> (≡)) (has_substate).
+  Proof.
+    intros ???.
+    unfold has_substate.
+    do 2 f_equiv.
+    intros i.
+    unfold of_idx, weakestpre.of_idx.
+    destruct (decide (i = sR_idx)).
+    - subst; simpl.
+      now do 3 f_equiv.
+    - reflexivity.
+  Qed.
 
   #[export] Instance state_interp_ne `{!stateG Σ} : NonExpansive state_interp.
   Proof. solve_proper. Qed.
